src/FS/MailServerAPI.v
@@ -7,6 +7,7 @@ Import ListNotations.
 Require Import String.
 Require Import FSAPI.
 
+
 Definition maildir := ["/tmp/"%string; "mail/"%string].
 Definition tmpdir := ["/tmp/"%string].
 
@@ -20,7 +21,8 @@ Definition starts_with_tid tid (name : string) : Prop :=
     name = (tid_to_string tid ++ "." ++ namesuffix)%string.
 
 Axiom starts_with_tid_not_dot : forall tid name,
-  starts_with_tid tid name -> name <> ".".
+    starts_with_tid tid name -> name <> ".".
+
 Axiom starts_with_tid_not_dotdot : forall tid name,
   starts_with_tid tid name -> name <> "..".
 
@@ -57,7 +59,7 @@ Inductive mailfs_step_allowed : forall T, fsOpT T -> nat -> Prop :=
 *)
 
 Definition invariant (fs : FS) :=
-  unique_pathname fs tmpdir.
+  unique_pathname_root fs tmpdir.
 
 Definition mailfs_step T (op : fsOpT T) tid s r s' :=
   fs_step_equiv op tid s r s' /\
@@ -108,13 +110,18 @@ Instance invariant_proper :
   Proper (FSEquiv ==> iff) invariant.
 Proof.
   intros ? ? ?; subst.
-  unfold invariant, unique_pathname; intuition; repeat deex.
-  - rewrite <- H in *.
-    eauto.
-  - specialize (H0 node node').
-    rewrite H in H1.
-    rewrite H in H2.
-    specialize (H0 H1 H2); auto.
+  unfold invariant, unique_pathname_root; intuition idtac; repeat deex.
+  - exists node.
+    rewrite <- H in *.
+    split; auto.
+    intros.
+    rewrite <- H in *.
+    auto.
+  - eexists node.
+    rewrite H in *.
+    split; auto.
+    intros.
+    rewrite H in *; auto.
 Qed.
 
 Lemma path_eval_root_create: forall fs pn dirnum h name,
@@ -123,148 +130,81 @@ Lemma path_eval_root_create: forall fs pn dirnum h name,
     path_eval_root (create_file dirnum h name fs) pn (DirNode dirnum ).
 Proof.
   intros.
-  eapply path_eval_root_updfile in H0.
-  eapply path_eval_root_addlink in H0; eauto.
+  eapply path_eval_root_upd_file in H0.
+  eapply path_eval_root_add_link in H0; eauto.
 Qed.
 
-Lemma valid_link_addlink_does_not_exists: forall fs dirnum name h node' node'' startdir name0,
-    name <> "." ->
-    name <> ".." ->
-    does_not_exist fs dirnum name ->
-    valid_link fs startdir name0 node'' ->
-    valid_link (add_link dirnum (FileNode h) name fs) startdir name0 node' ->
-    valid_link fs startdir name0 node'.
-Proof.
-  intros.
-  inversion H3; subst.
-  apply Graph.add_spec in H4.
-  intuition; subst. 
-  inversion H5; subst. clear H5.
-  destruct H1.
-  eexists.
-  inversion H2; subst; eauto; try congruence.
-  apply ValidDot.
-  eapply ValidDotDot.
-  apply Graph.add_spec in H4.
-  intuition; subst; try congruence.
-  eauto.
-  eapply ValidDotDotRoot.
-  unfold add_link; simpl; auto.
-Qed.
-
-Lemma path_eval_addlink' : forall fs dirpn startdir dirnum h name node,
-    name <> "." ->
-    name <> ".." ->
-     (forall node node' : Node,
-       path_evaluates fs (DirNode startdir) dirpn node ->
-       path_evaluates fs (DirNode startdir) dirpn node' -> node' = node) ->
-    does_not_exist fs dirnum name ->
-    path_evaluates fs (DirNode startdir) dirpn (DirNode dirnum) ->
-    path_evaluates (add_link dirnum (FileNode h) name fs) (DirNode startdir) dirpn node ->
-    DirNode dirnum = node.
-Proof.
-  intros.
-  generalize dependent fs; intros.
-  induction H3.
-  + inversion H4; subst; auto.
-  + inversion H4; subst; clear H4.
-    eapply valid_link_addlink_does_not_exists in H8; eauto.
-    inversion H11; subst.
-    eapply valid_link_addlink_does_not_exists in H9; eauto.
-    inversion H12; subst; clear H12.
-    eapply valid_link_addlink_does_not_exists in H9; eauto.
-    exfalso. admit.
-  + inversion H4; subst; clear H4.
-    eapply valid_link_addlink_does_not_exists in H11; eauto.
-    {
-      eapply valid_link_addlink_does_not_exists in H10; eauto.
-      assert (inum = inum0).
-      admit.
-      subst.
-      apply IHpath_evaluates; try eassumption.
-      admit.
-    }
-    { 
-      eapply valid_link_addlink_does_not_exists in H10; eauto.
-      admit.  (* H10 and H3 and H1 *)
-    }
-  + inversion H4; subst. clear H4.
-    eapply valid_link_addlink_does_not_exists in H10; eauto.
-    {
-      eapply valid_link_addlink_does_not_exists in H9; eauto.
-      admit.  (* H9 and H3 and H1 *)
-    }
-    eapply valid_link_addlink_does_not_exists in H9; eauto.
-    assert (sympath0 = sympath).
-    admit.
-    subst.
-    assert (symtarget = node).
-    subst.
-    eapply IHpath_evaluates1.
-    admit.
-    auto.
-    assert (node = symtarget0).
-    admit.
-    subst.
-    auto.
-    apply IHpath_evaluates2; auto.
-    admit.
-    assert (symtarget0 = symtarget).
-    admit.
-    subst.
-    auto.
- Admitted.
-
-Lemma path_eval_root_addlink' : forall fs dirnum name dirpn h node,
-    name <> "." ->
-    name <> ".." ->
-    does_not_exist fs dirnum name ->
-    unique_pathname fs dirpn ->
-    path_eval_root fs dirpn (DirNode dirnum) ->
-    path_eval_root (add_link dirnum (FileNode h) name fs) dirpn node ->
-    DirNode dirnum = node.
-Proof.
-  unfold unique_pathname, path_eval_root.
-  intros.
-  eapply path_eval_addlink'; try eassumption.
-Qed.
-
-Lemma path_eval_root_create': forall fs pn node dirnum h name,
-    name <> "." ->
-    name <> ".." ->
-    does_not_exist fs dirnum name ->
-    unique_pathname fs pn ->
-    path_eval_root fs pn (DirNode dirnum) ->
-    path_eval_root (create_file dirnum h name fs) pn node ->
-    DirNode dirnum = node.
-Proof.
-  intros.
-  unfold create_file in *.
-  eapply path_eval_root_updfile with (h := h) (data := "") in H3.
-  eapply path_eval_root_addlink' with (fs := (upd_file h "" fs)); try eassumption.
-  unfold upd_file; simpl.
-  admit.
+(*
+Lemma FS_path_evaluates_eq: forall fs fs' startdir pn node node',
+    FSEquiv fs fs' ->
+    path_evaluates fs (DirNode startdir) pn node ->
+    path_evaluates fs' (DirNode startdir) pn node' ->
+    node = node'.
 Admitted.
 
+Require Import Bool.
+Require Import Ascii.
+
+Definition eq_ascii (a1 a2 : ascii) :=
+  match a1, a2 with
+  | Ascii b1 b2 b3 b4 b5 b6 b7 b8, Ascii c1 c2 c3 c4 c5 c6 c7 c8 =>
+    (eqb b1 c1) && (eqb b2 c2) && (eqb b3 c3) && (eqb b4 c4) &&
+    (eqb b5 c5) && (eqb b6 c6) && (eqb b7 c7) && (eqb b8 c8)
+  end.
+
+Fixpoint eq_string (s1 s2 : string) :=
+  match s1, s2 with
+  | EmptyString,  EmptyString  => true
+  | String x1 s1, String x2 s2 => eq_ascii x1 x2 && eq_string s1 s2
+  | _, _                       => false
+  end.
+
+Definition match_dirent from s l :=
+  eq_string s (LinkName l) && (beq_nat from (LinkFrom l)).
+
+Definition dirents fs from name :=
+  Graph.filter (match_dirent from name) fs.
+
+Definition chooseone dirents := Graph.choose dirents.
+
+Fixpoint path pn (fs:Graph.t) dir: Graph.t :=
+  match pn with
+  | nil => Graph.empty
+  | e :: pn' =>
+    let s := dirents fs dir e in
+    match chooseone s with
+    | None => Graph.empty
+    | Some l =>
+      match (LinkTo l) with
+      | DirNode n => Graph.add l (path pn' fs n)
+        (* XXX symbolic links *)                      
+      | _ => Graph.empty
+      end
+    end
+  end.
+ *)
+
 Lemma path_unique_eq: forall fs dirnum pn node',
-    unique_pathname fs pn ->
+    unique_pathname_root fs pn ->
     path_eval_root fs pn (DirNode dirnum) ->
     path_eval_root fs pn node' ->
     node' = DirNode dirnum.
 Proof.
   intros.
-  unfold unique_pathname in *.
-  specialize (H (DirNode dirnum) node').
-  specialize (H H0 H1).
-  auto.
+  unfold unique_pathname_root in *.
+  deex.
+  specialize (H2 (DirNode dirnum)) as Hx.
+  specialize (Hx H0).
+  subst.
+  specialize (H2 node' H1); auto.
 Qed.
 
 Lemma path_unique_create_inum_eq: forall fs pn dirnum dirnum0 h name,
-    unique_pathname fs pn ->
+    unique_pathname_root fs pn ->
     does_not_exist fs dirnum0 name ->
     file_handle_unused fs h ->
     file_handle_valid fs h ->
-    unique_pathname (create_file dirnum0 h name fs) pn ->
+    unique_pathname_root (create_file dirnum0 h name fs) pn ->
     path_eval_root fs pn (DirNode dirnum0) ->
     path_eval_root (create_file dirnum0 h name fs) pn (DirNode dirnum) ->
     dirnum = dirnum0.
@@ -276,53 +216,243 @@ Proof.
   inversion Hinum; auto.
 Qed.
 
-Lemma invariant_create : forall fs pn dirnum h name,
-    name <> "." ->
-    name <> ".." ->
-    unique_pathname fs pn ->
-    does_not_exist fs dirnum name ->
-    file_handle_unused fs h ->
-    file_handle_valid fs h ->
-    path_eval_root fs pn (DirNode dirnum) ->
-    unique_pathname (create_file dirnum h name fs) pn.
+Lemma path_evaluates_add_link_upd_file : forall fs startdir node h data dirpn from to name,
+    path_evaluates (add_link from to name fs) startdir dirpn node ->
+    path_evaluates (add_link from to name (upd_file h data fs)) startdir dirpn node.
 Proof.
   intros.
-  unfold unique_pathname.
-  intros.
-  assert (DirNode dirnum = node).
-  eapply path_eval_root_create' in H6; try eassumption.
-  subst.
-  symmetry.
-  eapply path_eval_root_create' in H7; try eassumption.
+  remember (add_link from to name fs).
+  generalize dependent fs; intros.
+  induction H.
+  + constructor.
+  + eapply PathEvalFileLink; eauto.
+    inversion H; subst; clear H.
+    - constructor; simpl; auto.
+  + eapply PathEvalDirLink; eauto.
+    inversion H; subst; clear H.
+    - constructor; simpl; auto.
+    - apply ValidDot.
+    - eapply ValidDotDot; simpl; eauto.
+    - apply ValidDotDotRoot; auto.
+  + eapply PathEvalSymlink; subst; simpl.
+    inversion H; subst; clear H.
+    constructor; simpl; eauto.
+    apply IHpath_evaluates1; eauto.
+    apply IHpath_evaluates2; eauto.
 Qed.
 
-Lemma create_file_comm: forall fs dirnum h0 h1 name1 name0,
+Lemma path_evaluates_add_link_upd_file' : forall fs startdir node h data dirpn from to name,
+    path_evaluates (add_link from to name (upd_file h data fs)) startdir dirpn node ->
+    path_evaluates (add_link from to name fs) startdir dirpn node.
+Proof.
+  intros.
+  remember (add_link from to name (upd_file h data fs)).
+  generalize dependent fs; intros.
+  induction H.
+  + constructor.
+  + eapply PathEvalFileLink; eauto.
+    inversion H; subst; clear H.
+    - constructor; simpl; auto.
+  + eapply PathEvalDirLink; eauto.
+    inversion H; subst; clear H.
+    - constructor; simpl; auto.
+    - apply ValidDot.
+    - eapply ValidDotDot; simpl; eauto.
+    - apply ValidDotDotRoot; auto.
+  + eapply PathEvalSymlink; subst; simpl.
+    inversion H; subst; clear H.
+    constructor; simpl; eauto.
+    apply IHpath_evaluates1; eauto.
+    apply IHpath_evaluates2; eauto.
+Qed.
+
+Lemma path_evaluates_add_link_comm: forall fs pn startdir dirnum0 name2 n1 name1 n2 node,
+    path_evaluates (add_link dirnum0 n1 name1 (add_link dirnum0 n2 name2 fs)) (DirNode startdir) pn node ->
+    path_evaluates (add_link dirnum0 n2 name2 (add_link dirnum0 n1 name1 fs)) (DirNode startdir) pn node.
+Proof.
+  intros.
+  remember ((add_link dirnum0 n1 name1 (add_link dirnum0 n2 name2 fs))).
+  generalize dependent fs; intros.
+  induction H; subst.
+  + constructor.
+  + apply PathEvalFileLink; subst.
+    inversion H; subst; clear H.
+    constructor; simpl in *.
+    apply In_add_add_comm; auto.
+  + eapply PathEvalDirLink; eauto.
+    inversion H; subst; clear H.
+    - constructor; auto.
+      apply In_add_add_comm; auto.
+    - apply ValidDot.
+    - eapply ValidDotDot.
+      apply In_add_add_comm; eauto.
+    - apply ValidDotDotRoot; auto.
+  + inversion H; subst.
+    eapply PathEvalSymlink; simpl.
+    - constructor; simpl in *.
+      apply In_add_add_comm; auto.
+      apply H2.
+    - apply IHpath_evaluates1; eauto.
+    - apply IHpath_evaluates2; eauto.
+Qed.
+
+Lemma path_evaluates_add_link_add_link_upd_file: forall fs startdir dirnum0 node node0 node1 name0 name1 h data pn,
+   path_evaluates
+        (add_link dirnum0 node0 name0 (add_link dirnum0 node1 name1 (upd_file h data fs))) startdir pn node ->
+   path_evaluates
+     (add_link dirnum0 node0 name0 (add_link dirnum0 node1 name1 fs)) startdir pn node.
+Proof.
+  intros.
+  remember (add_link dirnum0 node0 name0 (add_link dirnum0 node1 name1 (upd_file h data fs))).
+  generalize dependent fs; intros.
+  induction H; subst.
+  + constructor.
+  + eapply PathEvalFileLink; eauto.
+    inversion H; subst; clear H.
+    - constructor; simpl; auto.
+  + eapply PathEvalDirLink; eauto.
+    inversion H; subst; clear H.
+    - constructor; simpl; auto.
+    - apply ValidDot.
+    - eapply ValidDotDot; simpl; eauto.
+    - apply ValidDotDotRoot; auto.
+  + eapply PathEvalSymlink; subst; simpl.
+    inversion H; subst; clear H.
+    constructor; simpl; eauto.
+    apply IHpath_evaluates1; eauto.
+    apply IHpath_evaluates2; eauto.
+Qed.
+
+Lemma path_evaluates_add_link_add_link_upd_file': forall fs startdir dirnum0 node node0 node1 name0 name1 h data pn,
+   path_evaluates
+     (add_link dirnum0 node0 name0 (add_link dirnum0 node1 name1 fs)) startdir pn node ->
+   path_evaluates
+        (add_link dirnum0 node0 name0 (add_link dirnum0 node1 name1 (upd_file h data fs))) startdir pn node.
+Proof.
+  intros.
+  remember (add_link dirnum0 node0 name0 (add_link dirnum0 node1 name1 fs)).
+  generalize dependent fs; intros.
+  induction H; subst.
+  + constructor.
+  + eapply PathEvalFileLink; eauto.
+    inversion H; subst; clear H.
+    - constructor; simpl; auto.
+  + eapply PathEvalDirLink; eauto.
+    inversion H; subst; clear H.
+    - constructor; simpl; auto.
+    - apply ValidDot.
+    - eapply ValidDotDot; simpl; eauto.
+    - apply ValidDotDotRoot; auto.
+  + eapply PathEvalSymlink; subst; simpl.
+    inversion H; subst; clear H.
+    constructor; simpl; eauto.
+    apply IHpath_evaluates1; eauto.
+    apply IHpath_evaluates2; eauto.
+Qed.
+
+Lemma path_evaluates_create_comm: forall fs pn startdir dirnum0 name0 v0 name1 v1 node,
+    path_evaluates (create_file dirnum0 v0 name0 (create_file dirnum0 v1 name1 fs)) (DirNode startdir) pn node ->
+    path_evaluates (create_file dirnum0 v1 name1 (create_file dirnum0 v0 name0 fs)) (DirNode startdir) pn node.
+Proof.
+  intros.
+  unfold create_file in *.
+  simpl in *.
+  eapply path_evaluates_add_link_upd_file.
+  eapply path_evaluates_add_link_upd_file' in H.
+  eapply path_evaluates_add_link_add_link_upd_file in H.
+  eapply path_evaluates_add_link_add_link_upd_file'.
+  apply path_evaluates_add_link_comm; auto.
+Qed.
+
+Lemma path_eval_root_create_comm: forall fs pn dirnum0 name v0 name0 v1 node,
+    path_eval_root (create_file dirnum0 v1 name0 (create_file dirnum0 v0 name fs)) pn node ->
+    path_eval_root (create_file dirnum0 v0 name (create_file dirnum0 v1 name0 fs)) pn node.
+Proof.
+  intros.
+  unfold path_eval_root in *.
+  eapply path_evaluates_create_comm; eauto.
+Qed.
+
+Lemma unique_pathname_create_comm: forall fs pn dirnum0 name v0 name0 v1,
+    unique_pathname_root (create_file dirnum0 v1 name0 (create_file dirnum0 v0 name fs)) pn ->
+    unique_pathname_root (create_file dirnum0 v0 name (create_file dirnum0 v1 name0 fs)) pn.
+Proof.
+  intros.
+  unfold unique_pathname_root in H.
+  unfold unique_pathname_root.
+  deex.
+  exists node.
+  split; auto.
+  eapply path_evaluates_create_comm; try eassumption.
+  intros.
+  specialize (H0 node'); auto.
+  edestruct H0.
+  eapply path_evaluates_create_comm; try eassumption.
+  reflexivity.
+Qed.  
+
+Lemma invariant_create_comm: forall fs dirnum0 name v0 name0 v1,
+    invariant (create_file dirnum0 v1 name0 (create_file dirnum0 v0 name fs)) ->
+    invariant (create_file dirnum0 v0 name (create_file dirnum0 v1 name0 fs)).
+Proof.
+  intros.
+  unfold invariant in *.
+  eapply unique_pathname_create_comm; eauto.
+Qed.
+
+Lemma unique_pathname_create: forall fs pn dirnum name1 v1,
+    unique_pathname_root fs pn ->
+    path_eval_root fs pn (DirNode dirnum) ->
+    unique_pathname_root (create_file dirnum v1 name1 fs) pn.
+Proof.
+  intros.
+  unfold unique_pathname_root, unique_pathname in *.
+  repeat deex.
+  unfold create_file, path_eval_root in *.
+  eexists.
+  split.
+  eapply path_evaluates_add_link_upd_file; simpl.
+  eapply path_evaluates_add_link in H as Hx.
+  apply Hx.
+
+  intros.
+  eapply H1.
+  eapply path_evaluates_add_link_upd_file' in H2.
+  apply path_evaluates_add_link' in H2; simpl in *; eauto.
+  unfold unique_pathname.
+  eexists.
+  split; eauto.
+  intros.
+  specialize (H1 node'0 H3) as H1x; subst.
+  symmetry.
+  specialize (H1 (DirNode dirnum) H0) as H1x; subst; auto.
+Admitted.
+
+Lemma invariant_create: forall fs dirnum name1 v1,
+    path_eval_root fs tmpdir (DirNode dirnum) ->
+    invariant fs ->
+    invariant (create_file dirnum v1 name1 fs).
+Proof.
+  intros.
+  unfold invariant in *.
+  eapply unique_pathname_create; eauto.
+Qed.
+
+Lemma fsequiv_create_file_comm: forall fs dirnum h0 h1 name1 name0,
     file_handle_unused fs h0 ->
     file_handle_unused (create_file dirnum h0 name0 fs) h1 ->
     FSEquiv (create_file dirnum h1 name1 (create_file dirnum h0 name0 fs))
             (create_file dirnum h0 name0 (create_file dirnum h1 name1 fs)).
 Proof.
   intros.
-  unfold create_file, add_link, upd_file, FSEquiv; simpl.
+  unfold create_file, FSEquiv; simpl.
   destruct fs; simpl.
   intuition eauto.
   eapply list_upd_commutes.
   eapply file_handle_unused_ne in H0 as Hx; eauto.
   unfold Graph.Equal; split; intros.
-  {
-    eapply Graph.add_spec in H1; intuition idtac; subst.
-    eapply Graph.add_spec; right. eapply Graph.add_spec; eauto.
-    eapply Graph.add_spec in H2; intuition idtac; subst.
-    eapply Graph.add_spec; eauto.
-    eapply Graph.add_spec; right. eapply Graph.add_spec; eauto.
-  }
-  {
-    eapply Graph.add_spec in H1; intuition idtac; subst.
-    eapply Graph.add_spec; right. eapply Graph.add_spec; eauto.
-    eapply Graph.add_spec in H2; intuition idtac; subst.
-    eapply Graph.add_spec; eauto.
-    eapply Graph.add_spec; right. eapply Graph.add_spec; eauto.
-  }
+  eapply In_add_add_comm; eauto.
+  eapply In_add_add_comm; eauto.
 Qed.
 
 Theorem create_tmpdir_both_mover : forall dir name,
@@ -344,7 +474,10 @@ Proof.
       econstructor; eauto.
       eauto.
 
-      apply invariant_create; try eauto.
+      eapply invariant_create; eauto.
+      
+      (* eapply invariant_create_comm in H11 as H11x; eauto. *)
+        
       (* some come from econstructor; others form invariant_create *)
       Unshelve.
       all: auto.
@@ -359,8 +492,9 @@ Proof.
       eauto.
       all: try unfold create_file; eauto.
 
-      apply create_file_comm; auto.
-      apply invariant_create; try eauto.
+      apply fsequiv_create_file_comm; auto.
+      eapply invariant_create_comm in H11 as H11x; eauto.
+      eapply invariant_create; eauto.
       Unshelve.
       all: auto.
 
